\documentclass[12pt]{article}
\newcommand{\diff}[0]{\, \mathrm{d}}
\usepackage[T1]{fontenc}
\usepackage{amsmath}
\everymath{\displaystyle}
\begin{document}
\section{Setup}
\[\frac{\partial T}{\partial t} + \nabla\cdot T \vec{u}-\alpha\nabla^2 T=q\]
\[\int_D (\frac{\partial T}{\partial t} + \nabla\cdot T \vec{u}-\alpha\nabla^2 T - q)\omega_i\diff x \diff t = 0\]
\vspace{3em}
%\[\psi_i(x) = 
%\begin{cases}
%1-\frac{x-x_{i-1}}{x_{i+1}-x_{i-1}} & x_{i-1} \leq x \leq x_i\\
%\frac{x-x_{i-1}}{x_{i+1}-x_{i-1}} & x_i \leq x \leq x_{i+1}\\
%\end{cases}\]
\[\psi_i(x) = 
\begin{cases}
\frac{x-x_{i-1}}{x_{i}-x_{i-1}} & x_{i-1} \leq x \leq x_i
\vspace{1ex}\\
\frac{-x-x_{i+1}}{x_{i+1}-x_i} & x_i \leq x \leq x_{i+1}\\
\end{cases}\]

\[\int_D (\frac{\partial T}{\partial t} + \frac{\partial{T\vec{u}}}{\partial t}+\frac{\partial T\vec{u}}{\partial{x}}+\frac{\partial^2 T}{\partial x^2}+\frac{\partial^2 T}{\partial t^2})\omega_i \diff x \diff t\]
\[\int_{t_k}^{t_{k+1}}\int_L (\frac{\partial T}{\partial t} + \frac{\partial{T\vec{u}}}{\partial t}+\frac{\partial T\vec{u}}{\partial{x}}+\frac{\partial^2 T}{\partial x^2}+\frac{\partial^2 T}{\partial t^2})\omega_i \diff x \diff t\]

\section{Transient Term}
\[\int_{t_k}^{t_{k+1}}\int_L \frac{\partial T}{\partial t} \omega_i \diff x \diff t \]
\[\int_D \frac{\partial T}{\partial t}\omega_i\diff x \diff t\]
\[\sum\limits_j\int_L \phi_jT_{j,k+1}\Delta t \omega_i\diff x\]
\[\sum\limits_jT_{j,k+1}\Delta t \int_L \phi_j\omega_i\diff x\]
\\
\[j=i-1\]
\[\sum\limits_j T_{j,k+1} \Delta t \frac{-x_{j-1}-5x_j}{6}\]
\[j=i\]
\[\sum\limits_jT_{j,k+1}\Delta t (x_{j+1}-x_{j-1})\]
\[j=i+1\]
\[\sum\limits_j T_{j,k+1} \Delta t \frac{-x_j-5x_{j+1}}{6}\]
\section{Convective Term}
\[\int_D \frac{\partial{T\vec{u}}}{\partial t}\omega_i+\frac{\partial T\vec{u}}{\partial x}\omega_i \diff x \diff t \]
\[\int_D \frac{\partial\sum\limits_j T_j\vec{u}\phi_j}{\partial t}\omega_i + \frac{\partial\sum\limits_j T_j\vec{u}\phi_j}{\partial x}\omega_i \diff x \diff t\]
\[\sum\limits_j T_{j,k+1} \vec{u}_{j,k+1} \Delta t \int_L  \phi_j+ \sum_j (x_{i+1}-x_{i-1})\int_t  T_j\vec{u}_j\phi_j \]
\end{document}