\documentclass[12pt]{article}
\newcommand{\diff}[0]{\, \mathrm{d}}
\usepackage[T1]{fontenc}
\usepackage{amsmath}
\everymath{\displaystyle}
\begin{document}
\[\frac{\partial T}{\partial t} + \nabla\cdot T \vec{u}-\alpha\nabla^2 T=q\]
\[\int_D (\frac{\partial T}{\partial t} + \nabla\cdot T \vec{u}-\alpha\nabla^2 T - q)\omega_i\diff x \diff t = 0\]
\vspace{3em}
\[\int_{t_0}^{t_1}\int_{x_w}^{x_e} \frac{\partial T}{\partial t} \omega_i\diff x \diff t\]
\[\phi_i(t) = 
\begin{cases}
1-\frac{t-t_{i-1}}{t_{i+1}-t_{i-1}} & t_{i-1} \leq t \leq t_i\\
\frac{t-t_{i-1}}{t_{i+1}-t_{i-1}} & t_i \leq t \leq t_{i+1}\\
\end{cases}\]
\[\psi_i(x) = 
\begin{cases}
1-\frac{x-x_{i-1}}{x_{i+1}-x_{i-1}} & x_{i-1} \leq x \leq x_i\\
\frac{x-x_{i-1}}{x_{i+1}-x_{i-1}} & x_i \leq x \leq x_{i+1}\\
\end{cases}\]
\[\sigma_i(x,y) = \psi_i(x)\phi_i(t)\]
\[\frac{\partial \sigma}{\partial t} = 
\begin{cases}
\frac{-\psi}{t_{i+1}-t_{i-1}} & t_{i-1} \leq t \leq t_i\\
\frac{\psi}{t_{i+1}-t_{i-1}} & t_i \leq t \leq t_{i+1}\\
\end{cases}\]
\[\frac{\partial \sigma}{\partial x} = 
\begin{cases}
\frac{-\phi}{x_{i+1}-x_{i-1}} & x_{i-1} \leq x \leq x_i\\
\frac{\phi}{x_{i+1}-x_{i-1}} & x_i \leq x \leq x_{i+1}\\
\end{cases}\]
\[\omega_i = \sigma_i\]

\[\int_D (\frac{\partial T}{\partial t} + \frac{\partial{T\vec{u}}}{\partial t}+\frac{\partial T\vec{u}}{\partial{x}}+\frac{\partial^2 T}{\partial x^2}+\frac{\partial^2 T}{\partial t^2})\omega_i \diff x \diff t\]
\end{document}